committed for martin

src/Convergence.thy
@@ -11,6 +11,7 @@ subsection\<open>Happens before relations and consistency\<close>
 locale happens_before = preorder hb_weak hb
   for hb_weak :: "'a \<Rightarrow> 'a \<Rightarrow> bool" and hb :: "'a \<Rightarrow> 'a \<Rightarrow> bool" +
   fixes interp :: "'a \<Rightarrow> 'b \<Rightarrow> 'b" ("\<langle>_\<rangle>" [100] 100)
+    and initial_state :: "'b"
 
 abbreviation (in happens_before) (input) concurrent :: "'a \<Rightarrow> 'a \<Rightarrow> bool" where
   "concurrent s1 s2 \<equiv> \<not> (hb s1 s2) \<and> \<not> (hb s2 s1)"
@@ -34,17 +35,48 @@ lemma (in happens_before) concurrent_set_Cons_Snoc [simp]:
   "concurrent_set a (xs@[x]) = concurrent_set a (x#xs)"
   by (auto simp: concurrent_set_def)
 
-definition (in happens_before) concurrent_elems_commute :: "'a list \<Rightarrow> bool" where
-  "concurrent_elems_commute xs \<equiv> (\<forall>x y. {x, y} \<subseteq> set xs \<and> concurrent x y \<longrightarrow> \<langle>x\<rangle> \<circ> \<langle>y\<rangle> = \<langle>y\<rangle> \<circ> \<langle>x\<rangle>)"
+inductive (in happens_before) concurrent_elems_commute :: "'a list \<Rightarrow> bool" where
+  [intro!]: "concurrent_elems_commute []" |
+  [intro]: "\<lbrakk> concurrent_elems_commute ops;
+     \<forall>x \<in> set ops. concurrent x y \<longrightarrow> (\<exists>ops1 ops2 s. ops = ops1@x#ops2 \<and>
+     s = fold (op \<circ>) (map interp ops1) id initial_state \<and>
+     (\<langle>x\<rangle> \<circ> \<langle>y\<rangle>) s = (\<langle>y\<rangle> \<circ> \<langle>x\<rangle>) s)
+   \<rbrakk> \<Longrightarrow> concurrent_elems_commute (ops@[y])"
 
-lemma (in happens_before) concurrent_elems_commute_ConsD [dest]:
-  assumes "concurrent_elems_commute (x # xs)"
-  shows   "concurrent_elems_commute xs"
-using assms by (auto simp: concurrent_elems_commute_def)
+(*
+inductive (in happens_before) concurrent_elems_commute :: "'a list \<Rightarrow> bool" where
+  [intro!]: "concurrent_elems_commute []" |
+  [intro!]: "concurrent_elems_commute [x]" |
+  [intro]: "\<lbrakk> concurrent_elems_commute (pre@[x]@mid);
+     concurrent x y;
+     s = fold (op \<circ>) (map interp pre) id initial_state;
+     (\<langle>x\<rangle> \<circ> \<langle>y\<rangle>) s = (\<langle>y\<rangle> \<circ> \<langle>x\<rangle>) s
+   \<rbrakk> \<Longrightarrow> concurrent_elems_commute (pre@x#mid@[y])"
+*)
 
+inductive_cases (in happens_before) concurrent_elems_commute_elim [elim]:
+  "concurrent_elems_commute []"
+  "concurrent_elems_commute [x]"
+  "concurrent_elems_commute (xs@[x])"
+  "concurrent_elems_commute xs"
+
+
+
+
+
+
+
+
+
+
+
+
+
+
+(*
 lemma (in happens_before) concurrent_elems_commute_ConsD2 [dest]:
   assumes "concurrent_elems_commute (x # y # xs)"
-  shows   "concurrent_elems_commute (x # xs) \<and> (concurrent x y \<longrightarrow> \<langle>x\<rangle> \<circ> \<langle>y\<rangle> = \<langle>y\<rangle> \<circ> \<langle>x\<rangle>)"
+  shows   "concurrent_elems_commute (x # xs) \<and> (\<forall>xs. P xs \<longrightarrow> concurrent x y \<longrightarrow> (\<langle>x\<rangle> \<circ> \<langle>y\<rangle>) xs = (\<langle>y\<rangle> \<circ> \<langle>x\<rangle>) xs)"
 using assms by (auto simp: concurrent_elems_commute_def)
 
 lemma (in happens_before) concurrent_elems_commute_Cons_eq [simp]:
@@ -52,23 +84,28 @@ lemma (in happens_before) concurrent_elems_commute_Cons_eq [simp]:
   by (auto simp: concurrent_elems_commute_def)
 
 lemma (in happens_before) concurrent_elems_commute_subset [intro]:
-  assumes "concurrent_elems_commute ys" "set xs \<subseteq> set ys"
-  shows   "concurrent_elems_commute xs"
+  assumes "concurrent_elems_commute ys P" "set xs \<subseteq> set ys"
+  shows   "concurrent_elems_commute xs P"
 using assms by (auto simp: concurrent_elems_commute_def)
+*)
 
 inductive (in happens_before) hb_consistent :: "'a list \<Rightarrow> bool" where
   [intro!]: "hb_consistent []" |
-  [intro!]: "\<lbrakk> hb_consistent xs; \<forall>x \<in> set xs. hb x y \<or> \<not> hb y x \<rbrakk> \<Longrightarrow> hb_consistent (xs @ [y])"
+  [intro!]: "\<lbrakk> hb_consistent xs; \<forall>x \<in> set xs. \<not> hb y x \<rbrakk> \<Longrightarrow> hb_consistent (xs @ [y])"
+
+lemma (in happens_before) "(hb x y \<or> concurrent x y) = (\<not> hb y x)"
+using local.less_asym by blast
 
 lemma (in happens_before) [intro!]:
   assumes "hb_consistent (xs @ ys)"
-  and     "\<forall>x \<in> set (xs @ ys). hb x z \<or> \<not> hb z x"
+  and     "\<forall>x \<in> set (xs @ ys). \<not> hb z x"
   shows   "hb_consistent (xs @ ys @ [z])"
 using assms hb_consistent.intros append_assoc by metis
 
 inductive_cases (in happens_before) hb_consistent_elim [elim]:
   "hb_consistent []"
   "hb_consistent (xs@[y])"
+  "hb_consistent (xs@ys)"
   "hb_consistent (xs@ys@[z])"
 
 inductive_cases (in happens_before) hb_consistent_elim_gen:
@@ -103,18 +140,37 @@ using hb_consistent.intros by fastforce
 
 lemma (in happens_before) fold_concurrent_rearrange:
   assumes "concurrent_set x xs"
-          "concurrent_elems_commute (x#xs)"
-  shows "\<langle>x\<rangle> \<circ> fold (op \<circ>) (map interp xs) id = fold (op \<circ>) (map interp xs) id \<circ> \<langle>x\<rangle>"
+          "concurrent_elems_commute (pre@x#xs)"
+  shows "(\<langle>x\<rangle> \<circ> fold (op \<circ>) (map interp xs) id) z = (fold (op \<circ>) (map interp xs) id \<circ> \<langle>x\<rangle>) z"
 using assms
   apply(induction xs rule: rev_induct, clarsimp)
+  apply clarsimp                   
+  apply(subgoal_tac "concurrent_elems_commute (x # xs) P")
+defer
+  apply(subst (asm) append_Cons[symmetric])
+  apply(subst (asm) concurrent_elems_commute_Cons_eq)
+  apply(drule concurrent_elems_commute_ConsD)
   apply clarsimp
-  apply(metis (no_types, hide_lams) append_Cons concurrent_elems_commute_ConsD concurrent_elems_commute_ConsD2 concurrent_elems_commute_Cons_eq o_assoc)
-done
+  apply clarsimp
+  apply(subgoal_tac "P (fold op \<circ> (map interp xs) id z)")
+  apply clarsimp
+  apply(subgoal_tac "((\<langle>x\<rangle>) \<circ> (\<langle>xa\<rangle>)) (fold op \<circ> (map interp xs) id z) = ((\<langle>xa\<rangle>) \<circ> (\<langle>x\<rangle>)) (fold op \<circ> (map interp xs) id z)")
+  apply clarsimp
+  apply(subst (asm) append_Cons[symmetric])
+  apply(subst (asm) concurrent_elems_commute_Cons_eq)
+  apply(drule concurrent_elems_commute_ConsD2)
+  apply auto
+  apply(subgoal_tac "P (fold op \<circ> (map interp xs) id z)")
+  apply presburger
+  apply(erule allE, erule impE, assumption)
+  
+(*  apply(metis (no_types, hide_lams) append_Cons concurrent_elems_commute_ConsD concurrent_elems_commute_ConsD2 concurrent_elems_commute_Cons_eq o_assoc)*)
+
 
 lemma (in happens_before) fold_concurrent_rearrange':
   assumes "concurrent_set x xs"
           "concurrent_elems_commute (x#xs)"
-  shows "fold (op \<circ>) (map interp (x#xs)) id = fold (op \<circ>) (map interp (xs@[x])) id"
+  shows "fold (op \<circ>) (map interp (pre@x#xs)) id = fold (op \<circ>) (map interp (pre@xs@[x])) id"
 using assms
   apply clarsimp
   apply(subst fold_concurrent_rearrange, clarsimp, clarsimp)
@@ -175,7 +231,7 @@ qed
 lemma (in happens_before) hb_consistent_append [intro!]:
   assumes "hb_consistent suffix"
           "hb_consistent prefix"
-          "\<And>s p. s \<in> set suffix \<Longrightarrow> p \<in> set prefix \<Longrightarrow> hb p s \<or> \<not> hb s p"
+          "\<And>s p. s \<in> set suffix \<Longrightarrow> p \<in> set prefix \<Longrightarrow> \<not> hb s p"
   shows "hb_consistent (prefix @ suffix)"
 using assms by (induction rule: hb_consistent.induct) force+
 
@@ -186,8 +242,108 @@ lemma (in happens_before) hb_consistent_append_porder:
   assumes "hb_consistent (xs @ ys)"
           "x \<in> set xs"
           "y \<in> set ys"
-  shows   "hb x y \<or> \<not> hb y x"
+  shows   "\<not> hb y x"
 using assms by (induction ys arbitrary: xs rule: rev_induct) force+
+
+lemma (in happens_before) " hb x y \<Longrightarrow> \<not> hb y x"
+apply (simp add: local.less_not_sym)
+done
+
+lemma (in happens_before) " concurrent x x"
+
+by simp
+
+lemma (in happens_before) foo:
+  shows "concurrent_elems_commute ops \<Longrightarrow>
+    concurrent_set x suffix \<Longrightarrow>
+    set (xs @ [x]) = set (prefix @ x # suffix) \<Longrightarrow>
+    ops = xs @ [x] \<Longrightarrow>
+    distinct (xs @ [x]) \<Longrightarrow>
+    distinct (prefix @ x # suffix) \<Longrightarrow> hb_consistent (xs @ [x]) \<Longrightarrow> hb_consistent(prefix @ x # suffix) \<Longrightarrow>
+    fold op \<circ> (map interp (prefix @ suffix @ [x])) id initial_state = fold op \<circ> (map interp (prefix @ x # suffix)) id initial_state"
+using assms
+  apply(induction arbitrary: prefix suffix x xs rule: concurrent_elems_commute.induct)
+  apply clarsimp
+
+apply (subgoal_tac "y = x \<and> ops = xs")
+prefer 2
+apply simp
+apply (subgoal_tac "ops = [] \<or> (\<exists>ox os. ops = os @ [ox])")
+apply (erule disjE)
+apply clarsimp
+apply (simp add: subset_insert)
+defer
+apply auto[1]
+
+apply (erule exE)+
+apply (subgoal_tac "ox \<in> set prefix \<or> ox \<in> set suffix")
+apply (erule disjE)
+
+apply (erule_tac x="prefix" in meta_allE)
+apply (erule_tac x=suffix in meta_allE)
+apply (erule_tac x=x in meta_allE)
+apply (erule_tac x=xs in meta_allE)
+
+
+
+
+
+oops
+theorem (in happens_before) convergence:
+  assumes "set xs = set ys"
+          "concurrent_elems_commute xs"
+          "distinct xs"
+          "distinct ys"
+          "hb_consistent xs"
+          "hb_consistent ys"
+  shows   "fold (op \<circ>) (map interp xs) id initial_state = fold (op \<circ>) (map interp ys) id initial_state"
+using assms proof(induction xs arbitrary: ys rule: rev_induct, simp)
+  fix x xs ys
+  assume IH: "(\<And>ys. set xs = set ys \<Longrightarrow>
+                    concurrent_elems_commute xs \<Longrightarrow> 
+                     distinct xs \<Longrightarrow> distinct ys \<Longrightarrow>
+                     hb_consistent xs \<Longrightarrow>
+                     hb_consistent ys \<Longrightarrow> 
+               fold op \<circ> (map interp xs) id initial_state = fold op \<circ> (map interp ys) id initial_state)"
+   assume assms: "set (xs @ [x]) = set ys"
+                 "concurrent_elems_commute (xs @ [x])"
+                 "distinct (xs @ [x])"      "distinct ys"
+                 "hb_consistent (xs @ [x])" "hb_consistent ys"
+  then obtain prefix suffix where ys_split: "ys = prefix @ x # suffix \<and> concurrent_set x suffix"
+    using hb_consistent_prefix_suffix_exists by fastforce
+  moreover have "distinct (prefix @ suffix)" "hb_consistent xs"
+    using ys_split assms by(auto simp add: disjoint_insert(1) distinct.simps(2) distinct_append list.simps(15))
+  moreover {
+    have "hb_consistent prefix" "hb_consistent suffix"
+      using ys_split assms by fastforce+
+    hence "hb_consistent (prefix @ suffix)"
+    using ys_split assms
+        apply clarsimp
+        apply(rule hb_consistent_append)
+        apply force apply force
+        apply(rule hb_consistent_append_porder)
+        apply(assumption) back
+        apply fastforce+
+      done
+  }
+  ultimately have IH': "fold op \<circ> (map interp xs) id initial_state = fold op \<circ> (map interp (prefix@suffix)) id initial_state"
+    using ys_split assms by (fastforce intro!: IH)
+  have "concurrent_elems_commute (prefix@suffix@[x])"
+    using ys_split assms sorry
+  have conc: "fold op \<circ> (map interp (prefix@suffix @ [x])) id initial_state = fold op \<circ> (map interp (prefix@x # suffix)) id initial_state"
+    using ys_split assms by(rule foo)
+  show "fold op \<circ> (map interp (xs @ [x])) id initial_state = fold op \<circ> (map interp ys) id initial_state"
+    apply (insert ys_split)
+    apply clarify
+    apply(subst conc[symmetric])
+    apply (subst map_append)
+    apply (subst fold_append)
+    apply (subst o_apply)
+    apply (subst fold_comp_eq)
+    apply (subst IH')
+    apply clarsimp
+  done
+qed
 
 theorem (in happens_before) convergence:
   assumes "set xs = set ys"
@@ -232,7 +388,7 @@ using assms proof(induction xs arbitrary: ys rule: rev_induct, simp)
   have "concurrent_elems_commute (x # suffix)"
     using ys_split assms concurrent_elems_commute_subset by auto
   have conc: "fold op \<circ> (map interp (suffix @ [x])) id = fold op \<circ> (map interp (x # suffix)) id"
-    using ys_split assms by (subst fold_concurrent_rearrange') auto
+    using ys_split assms by (subst fold_concurrent_rearrage') auto
   show "fold op \<circ> (map interp (xs @ [x])) id = fold op \<circ> (map interp ys) id"
     apply (insert ys_split)
     apply clarify
